\lecture{8}{26 Sep. 12:20}{}
Observe that 
\[
    \left\vert \frac{1}{\sqrt{5} } \left( \frac{1 - \sqrt{5} }{2} \right)^n  \right\vert < \frac{1}{2} .
\]
Hence, \(F_n\) is the integer closed to 
\[
    \frac{1}{\sqrt{5} } \left( \frac{1 + \sqrt{5} }{2} \right)^n. 
\] 

The idea is to encode a sequence of numbers 
\[
    a_0, a_1, a_2, \dots 
\]
as coefficients in a power series 
\[
    A(x) = \sum_{n=0}^{\infty} a_n x^n. 
\]

\begin{proposition}
    Let \((a_0, a_1, \dots )\) be a sequence of real numbers. If \(\vert a_n \vert < K^n \) for all \(n \in \mathbb{N} \), then
    \[
        \forall x \in \left( -\frac{1}{K}, \frac{1}{K} \right), \text{ we have } A(x) = \sum_{n=0}^{\infty} a_n x^n  
    \]  converges absolutely.
\end{proposition}
\begin{proof}
    Suppose \(x \in \left( -\frac{1}{K}, \frac{1}{K} \right) \), then 
    \[
        A(x) = \sum_{n=0}^{\infty} \left\vert a_n x^n \right\vert \le \sum_{n=0}^{\infty} \left\vert K^n x^n \right\vert = \sum_{n=0}^{\infty} \left( \left\vert Kx \right\vert  \right)^n,     
    \] which is a geometric series, and since \(\left\vert Kx \right\vert < 1 \), so it converges. 
\end{proof}

\(A(x)\) has derivatives of all orders at \(x = 0\), and for all \(n \ge 0\), 
    \[
        A^{(n)}(0) = a_n n!.
    \]  In particular, the values of \(A(x)\) around the origin determine this sequence \((a_n)\) uniquely. We treat \(A(x)\) as a formal power series.  Thus, we can usually eaily verigy results using induction. 

\begin{definition}
    Given a sequence \((a_0, a_1, \dots )\) of real numbers, the generating function of the sequence is the (formal) power series 
    \[
        \sum_{n=0}^{\infty} a_n x^n.  
    \]
\end{definition}

\begin{eg}
    Suppose we have a sequence \((1, 1, 1, \dots )\), then 
    \[
        A(x) = \sum_{n=0}^{\infty} x^n = \frac{1}{1-x} 
    \] converges for \(\vert x \vert < 1 \).  
\end{eg}

\begin{eg}
    Suppose we have a sequence \(\left( 0, 1, \frac{1}{2}, \dots  \right) \), then 
    \[
        A(x) = \sum_{n=0}^{\infty} \frac{x^n}{n} = -\ln (1 - x) 
    \] converges for \(\vert x \vert < 1 \).  
\end{eg}

\begin{eg}
    Suppose we have a sequence \(\left( 1, 1, \frac{1}{2}, \dots , \frac{1}{n!}, \dots  \right) \), then 
    \[
        A(x) = \sum_{n=0}^{\infty} \frac{x^n}{n!} = e^x
    \] converges for all \(x \in \mathbb{R} \).  
\end{eg}

\begin{eg}
    Suppose \(r\) is a fixed number and we have a sequence 
    \[
        \left( \binom{r}{0}, \binom{r}{1}, \dots  \right),
    \]then 
    \[
        A(x) = \sum_{n=0}^{\infty} \binom{r}{n} x^n = (1 + x)^r.  
    \] converges for \(\vert x \vert < 1 \).
\end{eg}

\begin{remark}
    The special case:
    \begin{align*}
        \frac{1}{(1 - x)^t} &= (1 - x)^{-t} = \sum_{n=0}^{\infty} \binom{-t}{n} (-x)^n = \sum_{n=0}^{\infty} \binom{-t}{n} (-1)^n x^n \\
        &= \sum_{n=0}^{\infty} \binom{t + n - 1}{n} x^n. 
    \end{align*}
\end{remark}

\section{Dictionary for operations}
\begin{itemize}
    \item Sum: 
    \begin{align*}
        A(x) &\sim (a_0, a_1, \dots ) \\
        B(x) &\sim (b_0, b_1, \dots ) \\
        A(x) + B(x) &\sim (a_0 + b_0, a_1 + b_1, \dots )
    \end{align*}
    \item Scalar multiplication: 
    \begin{align*}
        A(x) &\sim (a_0, a_1, \dots ) \\
        \lambda A(x) &\sim  (\lambda a_0, \lambda a_1, \dots ) \quad \forall \lambda > 0. 
    \end{align*}
    \item Shifting to the right:
    \begin{align*}
        (a_0, a_1, \dots ) &\sim \sum_{n=0}^{\infty} a_n x^n \\
        (0, a_0, a_1, \dots ) &\sim \sum_{n=1}^{\infty} a_{n-1} x^n = x \sum_{n=0}^{\infty} a_n x^n \\
        A(x) &\to x A(x)  
    \end{align*}
    \begin{note}
        By repeating shifting to the right, we can get 
        \[
            x^k A(x) \sim ( \underbrace{0,0, \dots ,0}_{k}, a_0, a_1, \dots  ).  
        \]
    \end{note}
    \item Shifting to the left: 
    \begin{align*}
        (a_0, a_1, \dots ) &\sim \sum_{n=0}^{\infty} a_n x^n \\
        (a_1, a_2 \dots ) &\sim \sum_{n=1}^{\infty} a_n x^{n-1} = \frac{A(x) - a_0}{x}.  
    \end{align*}
    \begin{note}
        By repeating 
        \[
            \frac{A(x) - a_0 - a_1 x - \dots - a_{k-1} x^{k-1}}{x^k},
        \] we can shift to the left by \(k\) terms. 
    \end{note}
    \item Substituting \(\lambda x\) for \(x\) with some \(\lambda \in \mathbb{R} \). 
    \begin{align*}
        A(\lambda x) &= \sum_{n=0}^{\infty} a_n \left( \lambda x \right)^n = \sum_{n=0}^{\infty} \left( a_n \lambda ^n \right) x^n     
    \end{align*}
    and it corresponds to \((a_0, \lambda a_1, \lambda ^2 a_2, \dots )\). 
\end{itemize}

\begin{eg}
    Suppose we want \((1, \lambda , \lambda ^2, \dots )\), then taking \((1, 1, \dots )\) and substituting \(x\) by \(\lambda x\), so we will change \(\frac{1}{1-x}\) to \(\frac{1}{1-\lambda x}\), and this means change \((1,1,\dots )\) to \((1, \lambda , \lambda ^2, \dots )\).     
\end{eg}
